Have duality.

Carrier/Lattice.thy
@@ -5,17 +5,17 @@ begin
 record 'a partial_object =
   carrier :: "'a set"
 
-abbreviation ftype :: "'a set \<Rightarrow> 'b set \<Rightarrow> ('a \<Rightarrow> 'b) set" (infixr "\<rightarrow>" 60) where
+definition ftype :: "'a set \<Rightarrow> 'b set \<Rightarrow> ('a \<Rightarrow> 'b) set" (infixr "\<rightarrow>" 60) where
   "ftype A B f \<equiv> (\<forall>x. x \<in> A \<longleftrightarrow> f x \<in> B)"
 
 lemma closed_composition: "\<lbrakk>f \<in> A \<rightarrow> B; g \<in> B \<rightarrow> C\<rbrakk> \<Longrightarrow> g \<circ> f \<in> A \<rightarrow> C"
-  by (simp add: mem_def)
+  by (simp add: mem_def ftype_def)
 
 lemma closed_application: "\<lbrakk>x \<in> A; f \<in> A \<rightarrow> B\<rbrakk> \<Longrightarrow> f x \<in> B"
-  by (simp add: mem_def)
+  by (simp add: mem_def ftype_def)
 
 lemma id_poly: "id \<in> A \<rightarrow> A"
-  by (simp add: mem_def)
+  by (simp add: mem_def ftype_def)
 
 locale equivalence = fixes S (structure)
   assumes refl [simp, intro]: "x \<in> carrier S \<Longrightarrow> x = x"
@@ -30,11 +30,37 @@ locale order = equivalence A for A (structure) +
   and order_trans: "\<lbrakk>x \<sqsubseteq> y; y \<sqsubseteq> z; x \<in> carrier A; y \<in> carrier A; z \<in> carrier A\<rbrakk> \<Longrightarrow> x \<sqsubseteq> z"
   and antisym: "\<lbrakk>x \<sqsubseteq> y; y \<sqsubseteq> x; x \<in> carrier A; y \<in> carrier A\<rbrakk> \<Longrightarrow> x = y"
 
+(* Inverse orders *)
+
+definition ord_inv :: "'a ord \<Rightarrow> 'a ord" ("_\<sharp>" [1000] 100) where
+  "ord_inv ordr \<equiv> \<lparr>carrier = carrier ordr, le = \<lambda>x y. le ordr y x\<rparr>"
+
+lemma inv_carrier_id [simp]: "carrier (ord_inv A) = carrier A"
+  by (metis ord_inv_def partial_object.simps(1))
+
+lemma ord_to_inv: "order A \<Longrightarrow> order (ord_inv A)"
+  by (default, simp_all add: ord_inv_def, (metis order.order_refl order.order_trans Lattice.order.antisym)+)
+
+lemma inv_inv_id: "ord_inv (ord_inv A) = A"
+  by (simp add: ord_inv_def)
+
+lemma inv_to_ord: "order (ord_inv A) \<Longrightarrow> order A"
+  by (metis inv_inv_id ord_to_inv)
+
+lemma ord_is_inv [simp]: "order (ord_inv A) = order A"
+  by (metis inv_to_ord ord_to_inv)
+
+lemma inv_flip [simp]: "(x \<sqsubseteq>\<^bsub>ord_inv A\<^esub> y) = (y \<sqsubseteq>\<^bsub>A\<^esub> x)"
+  by (simp add: ord_inv_def)
+
 definition isotone :: "'a ord \<Rightarrow> 'b ord \<Rightarrow> ('a \<Rightarrow> 'b) set" where
   "isotone A B f \<equiv> order A \<and> order B \<and> (\<forall>x\<in>carrier A. \<forall>y\<in>carrier A. x \<sqsubseteq>\<^bsub>A\<^esub> y \<longrightarrow> f x \<sqsubseteq>\<^bsub>B\<^esub> f y)"
 
 lemma use_iso1: "\<lbrakk>isotone A A f; x \<in> carrier A; y \<in> carrier A; x \<sqsubseteq>\<^bsub>A\<^esub> y\<rbrakk> \<Longrightarrow> f x \<sqsubseteq>\<^bsub>A\<^esub> f y"
   by (simp add: isotone_def)
+
+lemma inv_isotone [simp]: "isotone (A\<sharp>) (B\<sharp>) f = isotone A B f"
+  by (simp add: isotone_def, auto)
 
 definition idempotent :: "'a set \<Rightarrow> ('a \<Rightarrow> 'a) set" where
   "idempotent A f \<equiv> \<forall>x\<in>A. (f \<circ> f) x = f x"
@@ -52,11 +78,17 @@ begin
   definition is_lub :: "'a \<Rightarrow> 'a set \<Rightarrow> bool" where
     "is_lub x X \<equiv>  is_ub x X \<and> (\<forall>y\<in>carrier A.(\<forall>z\<in>X. z \<sqsubseteq> y) \<longrightarrow> x \<sqsubseteq> y)"
 
+  lemma is_lub_simp: "is_lub x X = ((X \<subseteq> carrier A) \<and> (x \<in> carrier A) \<and> (\<forall>y\<in>X. y \<sqsubseteq> x) \<and> (\<forall>y\<in>carrier A.(\<forall>z\<in>X. z \<sqsubseteq> y) \<longrightarrow> x \<sqsubseteq> y))"
+    by (simp add: is_lub_def is_ub_def)
+
   lemma is_lub_unique: "is_lub x X \<longrightarrow> is_lub y X \<longrightarrow> x = y"
     by (smt antisym is_lub_def is_ub_def)
 
   definition lub :: "'a set \<Rightarrow> 'a" ("\<Sigma>") where
     "\<Sigma> X = (THE x. is_lub x X)"
+
+  lemma lub_simp: "\<Sigma> X = (THE x. (X \<subseteq> carrier A) \<and> (x \<in> carrier A) \<and> (\<forall>y\<in>X. y \<sqsubseteq> x) \<and> (\<forall>y\<in>carrier A.(\<forall>z\<in>X. z \<sqsubseteq> y) \<longrightarrow> x \<sqsubseteq> y))"
+    by (simp add: lub_def is_lub_simp)
 
   lemma the_lub_leq: "\<lbrakk>\<exists>z. is_lub z X; \<And>z. is_lub z X \<longrightarrow> z \<sqsubseteq> x\<rbrakk> \<Longrightarrow> \<Sigma> X \<sqsubseteq> x"
     by (metis is_lub_unique lub_def the_equality)
@@ -90,11 +122,17 @@ begin
   definition is_glb :: "'a \<Rightarrow> 'a set \<Rightarrow> bool" where
     "is_glb x X \<longleftrightarrow> is_lb x X \<and> (\<forall>y\<in>carrier A.(\<forall>z\<in>X. y \<sqsubseteq> z) \<longrightarrow> y \<sqsubseteq> x)"
 
+  lemma is_glb_simp: "is_glb x X = ((X \<subseteq> carrier A) \<and> (x \<in> carrier A) \<and> (\<forall>y\<in>X. x \<sqsubseteq> y) \<and> (\<forall>y\<in>carrier A.(\<forall>z\<in>X. y \<sqsubseteq> z) \<longrightarrow> y \<sqsubseteq> x))"
+     by (simp add: is_glb_def is_lb_def)
+
   lemma is_glb_unique: "is_glb x X \<longrightarrow> is_glb y X \<longrightarrow> x = y"
     by (smt antisym is_glb_def is_lb_def)
 
   definition glb :: "'a set \<Rightarrow> 'a" ("\<Pi>") where
     "\<Pi> X = (THE x. is_glb x X)"
+
+  lemma glb_simp: "\<Pi> X = (THE x. (X \<subseteq> carrier A) \<and> (x \<in> carrier A) \<and> (\<forall>y\<in>X. x \<sqsubseteq> y) \<and> (\<forall>y\<in>carrier A.(\<forall>z\<in>X. y \<sqsubseteq> z) \<longrightarrow> y \<sqsubseteq> x))"
+    by (simp add: glb_def is_glb_simp)
 
   lemma the_glb_geq: "\<lbrakk>\<exists>z. is_glb z X; \<And>z. is_glb z X \<longrightarrow> x \<sqsubseteq> z\<rbrakk> \<Longrightarrow> x \<sqsubseteq> \<Pi> X"
     by (metis glb_def is_glb_unique the_equality)
@@ -120,17 +158,6 @@ begin
   definition meet :: "'a \<Rightarrow> 'a \<Rightarrow> 'a" (infixl "\<sqinter>" 70) where
     "x \<sqinter> y = \<Pi> {x,y}"
 
-  (* Duality of lubs and glbs *)
-
-  (*
-  lemma is_glb_from_is_lub: "\<lbrakk>X \<subseteq> carrier A; x \<in> carrier A; is_lub x {b. \<forall>a\<in>X. b \<sqsubseteq> a}\<rbrakk> \<Longrightarrow> is_glb x X"
-
-  lemma is_lub_from_is_glb: "\<lbrakk>is_glb x {b. \<forall>a\<in>A. a \<le> b}\<rbrakk> \<Longrightarrow> is_lub x A"
-    by (smt Collect_def is_lub_def is_ub_def is_glb_equiv mem_def order_refl)
-    *)
-
-  (* Join and meet preserving functions *)
-
 end
 
 abbreviation lub_ext :: "'a ord \<Rightarrow> 'a set \<Rightarrow> 'a" ("\<Sigma>\<^bsub>_\<^esub>_" [0,1000] 100) where
@@ -151,6 +178,17 @@ definition join_preserving :: "'a ord \<Rightarrow> 'b ord \<Rightarrow> ('a \<R
 definition meet_preserving :: "'a ord \<Rightarrow> 'b ord \<Rightarrow> ('a \<Rightarrow> 'b) \<Rightarrow> bool" where
   "meet_preserving A B g \<equiv> \<forall>X\<subseteq>carrier A. order.glb B (g ` X) = g (order.glb A X)"
 
+lemma dual_is_lub [simp]: "order A \<Longrightarrow> order.is_lub (A\<sharp>) x X = order.is_glb A x X"
+  by (simp add: order.is_glb_simp order.is_lub_simp)
+
+lemma dual_is_glb [simp]: "order A \<Longrightarrow> order.is_glb (A\<sharp>) x X = order.is_lub A x X"
+  by (simp add: order.is_glb_simp order.is_lub_simp)
+
+lemma dual_lub [simp]: "order A \<Longrightarrow> \<Sigma>\<^bsub>A\<sharp>\<^esub>X = \<Pi>\<^bsub>A\<^esub>X"
+  by (simp add: order.glb_simp order.lub_simp)
+
+lemma dual_glb [simp]: "order A \<Longrightarrow> \<Pi>\<^bsub>A\<sharp>\<^esub>X = \<Sigma>\<^bsub>A\<^esub>X"
+  by (simp add: order.glb_simp order.lub_simp)
 
 (* +------------------------------------------------------------------------+
    | Join semilattices                                                      |
@@ -276,6 +314,34 @@ begin
 
 end
 
+lemma inv_meet_semilattice_is_join [simp]: "meet_semilattice (A\<sharp>) = join_semilattice A"
+  by (simp_all add: meet_semilattice_def join_semilattice_def meet_semilattice_axioms_def join_semilattice_axioms_def, safe, simp_all)
+
+lemma inv_join_semilattice_is_meet [simp]: "join_semilattice (A\<sharp>) = meet_semilattice A"
+  by (simp add: meet_semilattice_def join_semilattice_def meet_semilattice_axioms_def join_semilattice_axioms_def, safe, simp_all)
+
+(* +------------------------------------------------------------------------+
+   | Lattices                                                               |
+   +------------------------------------------------------------------------+ *)
+
+locale lattice = join_semilattice + meet_semilattice
+
+begin
+
+  lemma absorb1: "\<lbrakk>x \<in> carrier A; y \<in> carrier A\<rbrakk> \<Longrightarrow> x \<squnion> (x \<sqinter> y) = x"
+    by (metis join_comm leq_def leq_meet_def meet_assoc meet_closed meet_comm meet_idem)
+
+  lemma absorb2: "\<lbrakk>x \<in> carrier A; y \<in> carrier A\<rbrakk> \<Longrightarrow> x \<sqinter> (x \<squnion> y) = x"
+    by (metis join_assoc join_closed join_comm join_idem leq_def leq_meet_def)
+
+  lemma order_change: "\<lbrakk>x \<in> carrier A; y \<in> carrier A\<rbrakk> \<Longrightarrow> x\<sqinter>y = y \<longleftrightarrow> y\<squnion>x = x"
+    by (metis leq_def leq_meet_def meet_comm)
+
+end
+
+lemma inv_lattice [simp]: "lattice (A\<sharp>) = lattice A"
+  by (simp add: lattice_def, auto)
+
 (* +------------------------------------------------------------------------+
    | Complete join semilattices                                             |
    +------------------------------------------------------------------------+ *)
@@ -316,25 +382,6 @@ begin
 
   lemma bot_onel [simp]: "\<lbrakk>x \<in> carrier A\<rbrakk> \<Longrightarrow> \<bottom> \<squnion> x = x"
     by (metis join_comm bot_oner)
-
-end
-
-(* +------------------------------------------------------------------------+
-   | Lattices                                                               |
-   +------------------------------------------------------------------------+ *)
-
-locale lattice = join_semilattice + meet_semilattice
-
-begin
-
-  lemma absorb1: "\<lbrakk>x \<in> carrier A; y \<in> carrier A\<rbrakk> \<Longrightarrow> x \<squnion> (x \<sqinter> y) = x"
-    by (metis join_comm leq_def leq_meet_def meet_assoc meet_closed meet_comm meet_idem)
-
-  lemma absorb2: "\<lbrakk>x \<in> carrier A; y \<in> carrier A\<rbrakk> \<Longrightarrow> x \<sqinter> (x \<squnion> y) = x"
-    by (metis join_assoc join_closed join_comm join_idem leq_def leq_meet_def)
-
-  lemma order_change: "\<lbrakk>x \<in> carrier A; y \<in> carrier A\<rbrakk> \<Longrightarrow> x\<sqinter>y = y \<longleftrightarrow> y\<squnion>x = x"
-    by (metis leq_def leq_meet_def meet_comm)
 
 end
 
@@ -381,6 +428,12 @@ begin
 
 end
 
+lemma inv_cms_is_cjs [simp]: "complete_meet_semilattice (A\<sharp>) = complete_join_semilattice A"
+  by (simp add: complete_meet_semilattice_def complete_join_semilattice_def complete_meet_semilattice_axioms_def complete_join_semilattice_axioms_def, safe, simp_all)
+
+lemma inv_cjs_is_cms [simp]: "complete_join_semilattice (A\<sharp>) = complete_meet_semilattice A"
+  by (simp add: complete_meet_semilattice_def complete_join_semilattice_def complete_meet_semilattice_axioms_def complete_join_semilattice_axioms_def, safe, simp_all)
+
 (* +------------------------------------------------------------------------+
    | Complete Lattices                                                      |
    +------------------------------------------------------------------------+ *)
@@ -395,6 +448,9 @@ lemma cl_to_cjs: "complete_lattice A \<Longrightarrow> complete_join_semilattice
 
 lemma cl_to_cms: "complete_lattice A \<Longrightarrow> complete_meet_semilattice A"
   by (simp add: complete_lattice_def)
+
+lemma inv_complete_lattice [simp]: "complete_lattice (A\<sharp>) = complete_lattice A"
+  by (simp add: complete_lattice_def, auto)
 
 sublocale complete_lattice \<subseteq> lattice
   by unfold_locales
@@ -416,17 +472,32 @@ definition is_pre_fp :: "'a ord \<Rightarrow> 'a \<Rightarrow> ('a \<Rightarrow>
 definition is_post_fp :: "'a ord \<Rightarrow> 'a \<Rightarrow> ('a \<Rightarrow> 'a) \<Rightarrow> bool" where
   "is_post_fp A x f \<equiv> order A \<and> f \<in> carrier A \<rightarrow> carrier A \<and> x \<in> carrier A \<and> x \<sqsubseteq>\<^bsub>A\<^esub> f x"
 
+lemma is_pre_fp_dual [simp]: "is_pre_fp (A\<sharp>) x f = is_post_fp A x f"
+  by (simp add: is_pre_fp_def is_post_fp_def)
+
+lemma is_post_fp_dual [simp]: "is_post_fp (A\<sharp>) x f = is_pre_fp A x f"
+  by (simp add: is_pre_fp_def is_post_fp_def)
+
 definition is_fp :: "'a ord \<Rightarrow> 'a \<Rightarrow> ('a \<Rightarrow> 'a) \<Rightarrow> bool" where
   "is_fp A x f \<equiv> order A \<and> f \<in> carrier A \<rightarrow> carrier A \<and> x \<in> carrier A \<and> f x = x"
 
+lemma is_fp_dual [simp]: "is_fp (A\<sharp>) x f = is_fp A x f"
+  by (simp add: is_fp_def)
+
 lemma is_fp_def_var: "is_fp A x f = (is_pre_fp A x f \<and> is_post_fp A x f)"
-  by (simp add: is_fp_def is_pre_fp_def is_post_fp_def, smt Lattice.order.antisym mem_def order.order_refl)
+  by (simp add: is_fp_def is_pre_fp_def is_post_fp_def, smt Lattice.order.antisym mem_def ftype_def order.order_refl)
 
 definition is_lpp :: "'a ord \<Rightarrow> 'a \<Rightarrow> ('a \<Rightarrow> 'a) \<Rightarrow> bool" where
   "is_lpp A x f \<equiv> (is_pre_fp A x f) \<and> (\<forall>y\<in>carrier A. f y \<sqsubseteq>\<^bsub>A\<^esub> y \<longrightarrow> x \<sqsubseteq>\<^bsub>A\<^esub> y)"
 
 definition is_gpp :: "'a ord \<Rightarrow> 'a \<Rightarrow> ('a \<Rightarrow> 'a) \<Rightarrow> bool" where
   "is_gpp A x f \<equiv> (is_post_fp A x f) \<and> (\<forall>y\<in>carrier A. y \<sqsubseteq>\<^bsub>A\<^esub> f y \<longrightarrow> y \<sqsubseteq>\<^bsub>A\<^esub> x)"
+
+lemma is_lpp_dual [simp]: "is_lpp (A\<sharp>) x f = is_gpp A x f"
+  by (simp add: is_gpp_def is_lpp_def)
+
+lemma is_gpp_dual [simp]: "is_gpp (A\<sharp>) x f = is_lpp A x f"
+  by (simp add: is_lpp_def is_gpp_def)
 
 definition is_lfp :: "'a ord \<Rightarrow> 'a \<Rightarrow> ('a \<Rightarrow> 'a) \<Rightarrow> bool" where
   "is_lfp A x f \<equiv> is_fp A x f \<and> (\<forall>y\<in>carrier A. is_fp A y f \<longrightarrow> x \<sqsubseteq>\<^bsub>A\<^esub> y)"
@@ -440,17 +511,35 @@ definition is_gfp :: "'a ord \<Rightarrow> 'a \<Rightarrow> ('a \<Rightarrow> 'a
 lemma is_gfp_closed: "is_gfp A x f \<Longrightarrow> f \<in> carrier A \<rightarrow> carrier A"
   by (metis (no_types) is_fp_def is_gfp_def)
 
+lemma is_lfp_dual [simp]: "is_lfp (A\<sharp>) x f = is_gfp A x f"
+  by (simp add: is_lfp_def is_gfp_def)
+
+lemma is_gfp_dual [simp]: "is_gfp (A\<sharp>) x f = is_lfp A x f"
+  by (simp add: is_gfp_def is_lfp_def)
+
 definition least_prefix_point :: "'a ord \<Rightarrow> ('a \<Rightarrow> 'a) \<Rightarrow> 'a" ("\<mu>\<^bsub>\<le>_\<^esub>_" [0,1000] 100) where
   "least_prefix_point A f \<equiv> THE x. is_lpp A x f"
 
 definition greatest_postfix_point :: "'a ord \<Rightarrow> ('a \<Rightarrow> 'a) \<Rightarrow> 'a" ("\<nu>\<^bsub>\<le>_\<^esub>_" [0,1000] 100) where
   "greatest_postfix_point A f \<equiv> THE x. is_gpp A x f"
 
+lemma least_prefix_point_dual [simp]: "\<mu>\<^bsub>\<le>(A\<sharp>)\<^esub>f = \<nu>\<^bsub>\<le>A\<^esub>f"
+  by (simp add: least_prefix_point_def greatest_postfix_point_def)
+
+lemma greatest_postfix_point_dual [simp]: "\<nu>\<^bsub>\<le>(A\<sharp>)\<^esub>f = \<mu>\<^bsub>\<le>A\<^esub>f"
+  by (simp add: least_prefix_point_def greatest_postfix_point_def)
+
 definition least_fixpoint :: "'a ord \<Rightarrow> ('a \<Rightarrow> 'a) \<Rightarrow> 'a" ("\<mu>\<^bsub>_\<^esub>_" [0,1000] 100) where
   "least_fixpoint A f \<equiv> THE x. is_lfp A x f"
 
 definition greatest_fixpoint :: "'a ord \<Rightarrow> ('a \<Rightarrow> 'a) \<Rightarrow> 'a" ("\<nu>\<^bsub>_\<^esub>_" [0,1000] 100) where
   "greatest_fixpoint A f \<equiv> THE x. is_gfp A x f"
+
+lemma least_fixpoint_dual [simp]: "\<mu>\<^bsub>(A\<sharp>)\<^esub>f = \<nu>\<^bsub>A\<^esub>f"
+  by (simp add: least_fixpoint_def greatest_fixpoint_def)
+
+lemma greatest_fixpoint_dual [simp]: "\<nu>\<^bsub>(A\<sharp>)\<^esub>f = \<mu>\<^bsub>A\<^esub>f"
+  by (simp add: least_fixpoint_def greatest_fixpoint_def)
 
 lemma lpp_unique: "\<lbrakk>is_lpp A x f; is_lpp A y f\<rbrakk> \<Longrightarrow> x = y"
   by (smt Lattice.order.antisym is_lpp_def is_pre_fp_def)
@@ -477,16 +566,16 @@ lemma gfp_equality_var [intro?]: "\<lbrakk>order A; f \<in> carrier A \<rightarr
   by (smt mem_def gfp_equality is_fp_def is_gfp_def)
 
 lemma lpp_is_lfp: "\<lbrakk>isotone A A f; is_lpp A x f\<rbrakk> \<Longrightarrow> is_lfp A x f"
-  by (simp add: isotone_def is_lpp_def is_pre_fp_def is_lfp_def is_fp_def, smt Lattice.order.antisym mem_def order.order_refl)
+  by (simp add: isotone_def is_lpp_def is_pre_fp_def is_lfp_def is_fp_def, smt Lattice.order.antisym mem_def order.order_refl ftype_def)
 
 lemma gpp_is_gfp: "\<lbrakk>isotone A A f; is_gpp A x f\<rbrakk> \<Longrightarrow> is_gfp A x f"
-  by (simp add: isotone_def is_gpp_def is_post_fp_def is_gfp_def is_fp_def, smt Lattice.order.antisym mem_def order.order_refl)
+  by (simp add: isotone_def is_gpp_def is_post_fp_def is_gfp_def is_fp_def, smt Lattice.order.antisym mem_def order.order_refl ftype_def)
 
 lemma least_fixpoint_set: "\<lbrakk>\<exists>x. is_lfp A x f\<rbrakk> \<Longrightarrow> \<mu>\<^bsub>A\<^esub> f \<in> carrier A"
   by (simp add: least_fixpoint_def, rule the1I2, metis lfp_equality, metis is_lfp_def is_fp_def)
 
 lemma greatest_fixpoint_set: "\<lbrakk>\<exists>x. is_gfp A x f\<rbrakk> \<Longrightarrow> \<nu>\<^bsub>A\<^esub> f \<in> carrier A"
-  by (simp add: greatest_fixpoint_def, rule the1I2, metis gfp_equality, metis is_fp_def is_gfp_def)
+  by (unfold is_lfp_dual[symmetric] least_fixpoint_dual[symmetric], metis inv_carrier_id least_fixpoint_set)
 
 (* +------------------------------------------------------------------------+
    | Knaster-Tarski for least fixed points                                  |
@@ -508,8 +597,8 @@ proof
   proof -
     have "\<forall>x\<in>?H. ?a \<sqsubseteq>\<^bsub>A\<^esub> x" by (smt H_carrier complete_meet_semilattice.glb_least cl_A cl_to_cms)
     hence "\<forall>x\<in>?H. f ?a \<sqsubseteq>\<^bsub>A\<^esub> f x" by (safe, rule_tac ?f = f in use_iso1, metis f_iso, metis a_carrier, auto)
-    hence "\<forall>x\<in>?H. f ?a \<sqsubseteq>\<^bsub>A\<^esub> x" by (smt Collect_def a_carrier cl_A cl_to_order f_closed mem_def order.order_trans)
-    hence "f ?a \<sqsubseteq>\<^bsub>A\<^esub> ?a" by (smt mem_def complete_meet_semilattice.glb_greatest Collect_def cl_A cl_to_cms a_carrier f_closed H_carrier)
+    hence "\<forall>x\<in>?H. f ?a \<sqsubseteq>\<^bsub>A\<^esub> x" by (smt Collect_def a_carrier cl_A cl_to_order f_closed mem_def order.order_trans ftype_def)
+    hence "f ?a \<sqsubseteq>\<^bsub>A\<^esub> ?a" by (smt mem_def complete_meet_semilattice.glb_greatest Collect_def cl_A cl_to_cms a_carrier f_closed H_carrier ftype_def)
     thus ?thesis by (smt a_carrier cl_A cl_to_order f_closed is_pre_fp_def mem_def)
   qed
   moreover show "\<And>x\<Colon>'a. is_lpp A x f \<Longrightarrow> x = ?a"
@@ -522,13 +611,13 @@ corollary is_lpp_lpp [intro?]:
   "\<lbrakk>complete_lattice A; f \<in> carrier A \<rightarrow> carrier A; isotone A A f\<rbrakk> \<Longrightarrow> is_lpp A (\<mu>\<^bsub>\<le>A\<^esub> f) f"
   by (smt knaster_tarski_lpp lpp_equality mem_def)
 
-theorem knaster_tarksi:
+theorem knaster_tarski:
   "\<lbrakk>complete_lattice A; f \<in> carrier A \<rightarrow> carrier A; isotone A A f\<rbrakk> \<Longrightarrow> \<exists>!x. is_lfp A x f"
   by (smt is_lpp_lpp lfp_equality lpp_is_lfp mem_def)
 
 corollary is_lfp_lfp [intro?]:
   "\<lbrakk>complete_lattice A; f \<in> carrier A \<rightarrow> carrier A; isotone A A f\<rbrakk> \<Longrightarrow> is_lfp A (\<mu>\<^bsub>A\<^esub> f) f"
-  by (smt knaster_tarksi lfp_equality mem_def)
+  by (smt knaster_tarski lfp_equality mem_def)
 
 (* +------------------------------------------------------------------------+
    | Knaster-Tarski for greatest fixed points                               |
@@ -538,39 +627,23 @@ theorem knaster_tarski_gpp:
   assumes cl_A: "complete_lattice A" and f_closed: "f \<in> carrier A \<rightarrow> carrier A"
   and f_iso: "isotone A A f"
   shows "\<exists>!x. is_gpp A x f"
-proof
-  let ?H = "{u. u \<sqsubseteq>\<^bsub>A\<^esub> f u \<and> u \<in> carrier A}"
-  let ?a = "\<Sigma>\<^bsub>A\<^esub>?H"
-
-  have H_carrier: "?H \<subseteq> carrier A" by (default, simp add: Collect_def mem_def)
-  hence a_carrier: "?a \<in> carrier A"
-    by (smt order.lub_closed complete_join_semilattice.is_lub_lub cl_A cl_to_cjs cl_to_order)
-
-  have "is_post_fp A ?a f"
-  proof -
-    have "\<forall>x\<in>?H. x \<sqsubseteq>\<^bsub>A\<^esub> ?a" by (smt H_carrier complete_join_semilattice.lub_least cl_A cl_to_cjs)
-    hence "\<forall>x\<in>?H. f x \<sqsubseteq>\<^bsub>A\<^esub> f ?a" by (safe, rule_tac ?f = f in use_iso1, metis f_iso, metis a_carrier, auto, metis a_carrier)
-    hence "\<forall>x\<in>?H. x \<sqsubseteq>\<^bsub>A\<^esub> f ?a" by (smt Collect_def a_carrier cl_A cl_to_order f_closed mem_def order.order_trans)
-    hence "?a \<sqsubseteq>\<^bsub>A\<^esub> f ?a" by (smt mem_def complete_join_semilattice.lub_greatest Collect_def cl_A cl_to_cjs a_carrier f_closed H_carrier)
-    thus ?thesis by (smt a_carrier cl_A cl_to_order f_closed is_post_fp_def mem_def)
-  qed
-  moreover show "\<And>x\<Colon>'a. is_gpp A x f \<Longrightarrow> x = ?a"
-    by (smt Collect_def H_carrier calculation cl_A cl_to_cjs complete_join_semilattice.lub_least is_gpp_def gpp_unique mem_def)
-  ultimately show "is_gpp A ?a f"
-    by (smt Collect_def H_carrier cl_A cl_to_cjs complete_join_semilattice.lub_least is_gpp_def mem_def)
+proof -
+  have dual: "\<lbrakk>complete_lattice (A\<sharp>); f \<in> carrier (A\<sharp>) \<rightarrow> carrier (A\<sharp>); isotone (A\<sharp>) (A\<sharp>) f\<rbrakk> \<Longrightarrow> \<exists>!x. is_lpp (A\<sharp>) x f"
+    by (smt knaster_tarski_lpp)
+  thus ?thesis by (simp, metis cl_A f_closed f_iso)
 qed
 
 corollary is_gpp_gpp [intro?]:
   "\<lbrakk>complete_lattice A; f \<in> carrier A \<rightarrow> carrier A; isotone A A f\<rbrakk> \<Longrightarrow> is_gpp A (\<nu>\<^bsub>\<le>A\<^esub> f) f"
   by (smt knaster_tarski_gpp gpp_equality mem_def)
 
-theorem knaster_tarksi_greatest:
+theorem knaster_tarski_greatest:
   "\<lbrakk>complete_lattice A; f \<in> carrier A \<rightarrow> carrier A; isotone A A f\<rbrakk> \<Longrightarrow> \<exists>!x. is_gfp A x f"
   by (smt is_gpp_gpp gfp_equality gpp_is_gfp mem_def)
 
 corollary is_gfp_gfp [intro?]:
   "\<lbrakk>complete_lattice A; f \<in> carrier A \<rightarrow> carrier A; isotone A A f\<rbrakk> \<Longrightarrow> is_gfp A (\<nu>\<^bsub>A\<^esub> f) f"
-  by (smt knaster_tarksi_greatest gfp_equality mem_def)
+  by (smt knaster_tarski_greatest gfp_equality mem_def)
 
 (* +------------------------------------------------------------------------+
    | Fixpoint Computation                                                   |
@@ -627,7 +700,7 @@ lemma fixpoint_compose:
   and x_carrier: "x \<in> carrier A" and k_iso: "isotone A A k"
   and comp: "g\<circ>k = k\<circ>h" and fp: "is_fp A x h"
   shows "is_fp A (k x) g"
-  using fp and comp by (simp add: is_fp_def o_def, safe, (smt mem_def g_closed k_closed)+)
+  using fp and comp by (simp add: is_fp_def o_def, safe, (metis g_closed k_closed closed_application)+)
 
 lemma fixpoint_mono:
   assumes cl_A: "complete_lattice A"
